@prefix owl: <http://www.w3.org/2002/07/owl#> .
@prefix pleiades: <http://pleiades.stoa.org/places/vocab#> .
@prefix rdf: <http://www.w3.org/1999/02/22-rdf-syntax-ns#> .
@prefix rdfs: <http://www.w3.org/2000/01/rdf-schema#> .
@prefix skos: <http://www.w3.org/2004/02/skos/core#> .
@prefix xsd: <http://www.w3.org/2001/XMLSchema#> .

pleiades:Place a rdfs:Class, owl:Class ;
    rdfs:label "Place"@en ;
    rdfs:comment "Places are instances of skos:Concept as well as contexts for Locations and Names."@en ;
    rdfs:subClassOf skos:Concept .

pleiades:Location a rdfs:Class, owl:Class ;
    rdfs:label "Location"@en ;
    rdfs:comment "Locations describe natural or man-made features of the real world."@en .

pleiades:Name a rdfs:Class, owl:Class ;
    rdfs:label "Name"@en ;
    rdfs:comment "Names describe appellations in the context of a Place."@en .

pleiades:hasLocation a rdf:Property, owl:ObjectProperty ;
    rdfs:label "has location"@en ;
    rdfs:domain pleiades:Place ;
    rdfs:range pleiades:Location .

pleiades:hasName a rdf:Property, owl:ObjectProperty ;
    rdfs:label "has name"@en ;
    rdfs:domain pleiades:Place ;
    rdfs:range pleiades:Location .

pleiades:during a rdf:Property, owl:ObjectProperty ;
    rdfs:label "during"@en ;
    rdfs:comment "Indicates that the entity was in use or active during a named time period from http://pleiades.stoa.org/vocabularies/time-periods."@en ;
    rdfs:range skos:Concept .

pleiades:start_date a rdf:Property, owl:DatatypeProperty ;
    rdfs:label "start date"@en ;
    rdfs:comment "Indicates the earliest date (CE year) of all related time periods."@en ;
    rdfs:range xsd:integer .

pleiades:end_date a rdf:Property, owl:DatatypeProperty ;
    rdfs:label "end date"@en ;
    rdfs:comment "Indicates the latest date (CE year) of all related time periods."@en ;
    rdfs:range xsd:integer .

pleiades:hasFeatureType a rdf:Property, owl:ObjectProperty ;
    rdfs:label "has feature type"@en ;
    rdfs:comment "Indicates that the entity had a certain feature type or category of use from http://pleiades.stoa.org/vocabularies/place-types."@en ;
    rdfs:range skos:Concept .

pleiades:nameAttested a rdf:Property, owl:DatatypeProperty ;
    rdfs:label "name attested"@en ;
    rdfs:comment "The attested form of a historical name in its own language and writing system."@en ;
    rdfs:domain pleiades:Name ;
    rdfs:range xsd:string .

pleiades:nameRomanized a rdf:Property, owl:DatatypeProperty ;
    rdfs:label "name romanized"@en ;
    rdfs:comment "A romanized or transliterated form of a historical name."@en ;
    rdfs:domain pleiades:Name ;
    rdfs:range xsd:string .

